[CBPV] Add proofs of soundness and completeness of CK machine semantics wrt small-step evaluation

CBPV/CK.lean
@@ -1,26 +1,46 @@
 import CBPV.RTC
 import CBPV.Syntax
+import CBPV.Evaluation
+
+namespace CK
 
 inductive F : Type where
   | app : Val → F
   | letin : Com → F
   | fst : F
   | snd : F
+open F
 
 def K := List F
 def CK := Com × K
+
+@[simp]
+def renameK (ξ : Nat → Nat) : K → K
+  | [] => []
+  | app v :: k => .app (renameVal ξ v) :: renameK ξ k
+  | letin m :: k => .letin (renameCom (lift ξ) m) :: renameK ξ k
+  | fst :: k => fst :: renameK ξ k
+  | snd :: k => snd :: renameK ξ k
+
+@[simp]
+def dismantle (n : Com) : K → Com
+  | [] => n
+  | app v :: k => dismantle (.app n v) k
+  | letin m :: k => dismantle (.letin n m) k
+  | fst :: k => dismantle (.fst n) k
+  | snd :: k => dismantle (.snd n) k
 
 section
 set_option hygiene false
 local infix:40 "⤳" => Step
 inductive Step : CK → CK → Prop where
   | β {m v k} :     ⟨.lam m, .app v :: k⟩   ⤳ ⟨substCom (v +: .var) m, k⟩
+  | ζ {v m k} :     ⟨.ret v, .letin m :: k⟩ ⤳ ⟨substCom (v +: .var) m, k⟩
   | ιl {v m n k} :  ⟨.case (.inl v) m n, k⟩ ⤳ ⟨substCom (v +: .var) m, k⟩
   | ιr {v m n k} :  ⟨.case (.inr v) m n, k⟩ ⤳ ⟨substCom (v +: .var) n, k⟩
   | π {m k} :       ⟨.force (.thunk m), k⟩  ⤳ ⟨m, k⟩
   | π1 {m n k} :    ⟨.prod m n, .fst :: k⟩  ⤳ ⟨m, k⟩
   | π2 {m n k} :    ⟨.prod m n, .snd :: k⟩  ⤳ ⟨n, k⟩
-  | ζ {v m k} :     ⟨.ret v, .letin m :: k⟩ ⤳ ⟨substCom (v +: .var) m, k⟩
   | app {m v k} :   ⟨.app m v, k⟩           ⤳ ⟨m, .app v :: k⟩
   | letin {m n k} : ⟨.letin m n, k⟩         ⤳ ⟨m, .letin n :: k⟩
   | fst {m k} :     ⟨.fst m, k⟩             ⤳ ⟨m, .fst :: k⟩
@@ -30,3 +50,156 @@ infix:40 "⤳" => Step
 
 @[reducible] def Steps := RTC Step
 infix:40 "⤳⋆"  => Steps
+
+end CK
+
+namespace Big
+
+section
+set_option hygiene false
+local infix:40 (priority := 1001) "⇓" => BStep
+inductive BStep : Com → Com → Prop where
+  | lam {m} : .lam m ⇓ .lam m
+  | ret {v} : .ret v ⇓ .ret v
+  | prod {m₁ m₂} : .prod m₁ m₂ ⇓ .prod m₁ m₂
+  | π {m t} :
+    m ⇓ t →
+    ---------------------
+    .force (.thunk m) ⇓ t
+  | β {n t m v} :
+    n ⇓ .lam m →
+    substCom (v +: .var) m ⇓ t →
+    -----------------------------
+    .app n v ⇓ t
+  | ζ {n t v m} :
+    n ⇓ .ret v →
+    substCom (v +: .var) m ⇓ t →
+    -----------------------------
+    .letin n m ⇓ t
+  | ιl {v m₁ m₂ t}:
+    substCom (v +: .var) m₁ ⇓ t →
+    -----------------------------
+    .case (.inl v) m₁ m₂ ⇓ t
+  | ιr {v m₁ m₂ t}:
+    substCom (v +: .var) m₂ ⇓ t →
+    -----------------------------
+    .case (.inr v) m₁ m₂ ⇓ t
+  | π1 {n t m₁ m₂} :
+    n ⇓ .prod m₁ m₂ →
+    m₁ ⇓ t →
+    -----------
+    .fst n ⇓ t
+  | π2 {n t m₁ m₂} :
+    n ⇓ .prod m₁ m₂ →
+    m₂ ⇓ t →
+    -----------
+    .snd n ⇓ t
+end
+infix:40 (priority := 1001) "⇓" => BStep
+
+@[simp]
+def isTerminal : Com → Prop
+  | .lam _ | .ret _ | .prod _ _ => True
+  | _ => False
+
+end Big
+
+open CK Big
+
+/-* CK machine semantics is sound wrt small-step evaluation semantics *-/
+
+theorem congK {m n k} (r : m ⇒ n) : dismantle m k ⇒ dismantle n k := by
+  induction k generalizing m n
+  case nil => simp [r]
+  case cons f _ ih =>
+    cases f
+    all_goals apply ih; constructor; apply r
+
+theorem stepEval {m n k₁ k₂} (r : ⟨m, k₁⟩ ⤳ ⟨n, k₂⟩) :
+  (dismantle m k₁ ⇒ dismantle n k₂) ∨ (dismantle m k₁ = dismantle n k₂) := by
+  generalize e₁ : (m, k₁) = ck₁ at r
+  generalize e₂ : (n, k₂) = ck₂ at r
+  induction r generalizing m n k₁ k₂
+  all_goals injection e₁ with em ek₁; subst em ek₁
+  all_goals injection e₂ with en ek₂; subst en ek₂
+  case β | ζ | ιl | ιr | π | π1 | π2 => (try simp); left; apply congK; constructor
+  case app | letin | fst | snd => right; rfl
+
+theorem stepEvals {m n k₁ k₂} (r : ⟨m, k₁⟩ ⤳⋆ ⟨n, k₂⟩) : dismantle m k₁ ⇒⋆ dismantle n k₂ := by
+  generalize e₁ : (m, k₁) = ck₁ at r
+  generalize e₂ : (n, k₂) = ck₂ at r
+  induction r generalizing m n k₁ k₂
+  case refl => subst e₁; injection e₂ with em ek; subst em ek; rfl
+  case trans ck _ r _ ih =>
+    subst e₁ e₂; cases ck; specialize ih rfl rfl
+    match stepEval r with
+    | .inl r => exact .trans r ih
+    | .inr e => simp [e, ih]
+
+theorem stepEvalsNil {m n} : ⟨m, []⟩ ⤳⋆ ⟨n, []⟩ → m ⇒⋆ n := stepEvals
+
+/-* CK machine semantics is complete wrt big-step semantics *-/
+
+theorem stepBig {m n k} (r : m ⇓ n) : ⟨m, k⟩ ⤳⋆ ⟨n, k⟩ := by
+  induction r generalizing k
+  case lam | ret | prod => rfl
+  case π ih => exact .trans .π ih
+  case ιl ih => exact .trans .ιl ih
+  case ιr ih => exact .trans .ιr ih
+  case β n t m v _ _ ih₁ ih₂ =>
+    calc ⟨.app n v, k⟩
+      _ ⤳  ⟨n, .app v :: k⟩      := .app
+      _ ⤳⋆ ⟨.lam m, .app v :: k⟩ := ih₁
+      _ ⤳  ⟨m⦃v⦄, k⟩             := .β
+      _ ⤳⋆ ⟨t, k⟩                := ih₂
+  case ζ n t v m _ _ ih₁ ih₂ =>
+    calc ⟨.letin n m, k⟩
+      _ ⤳  ⟨n, .letin m :: k⟩      := .letin
+      _ ⤳⋆ ⟨.ret v, .letin m :: k⟩ := ih₁
+      _ ⤳  ⟨m⦃v⦄, k⟩               := .ζ
+      _ ⤳⋆ ⟨t, k⟩                  := ih₂
+  case π1 n t m₁ m₂ _ _ ih₁ ih₂ =>
+    calc ⟨.fst n, k⟩
+      _ ⤳  ⟨n, .fst :: k⟩           := .fst
+      _ ⤳⋆ ⟨.prod m₁ m₂, .fst :: k⟩ := ih₁
+      _ ⤳  ⟨m₁, k⟩                  := .π1
+      _ ⤳⋆ ⟨t, k⟩                   := ih₂
+  case π2 n t m₁ m₂ _ _ ih₁ ih₂ =>
+    calc ⟨.snd n, k⟩
+      _ ⤳  ⟨n, .snd :: k⟩           := .snd
+      _ ⤳⋆ ⟨.prod m₁ m₂, .snd :: k⟩ := ih₁
+      _ ⤳  ⟨m₂, k⟩                  := .π2
+      _ ⤳⋆ ⟨t, k⟩                   := ih₂
+
+/-* CK machine is complete wrt small-step evaluation via big-step *-/
+
+theorem evalBig {m n t} (r : m ⇒ n) : n ⇓ t → m ⇓ t := by
+  induction r generalizing t <;> intro r
+  case π => exact .π r
+  case β => exact .β .lam r
+  case ζ => exact .ζ .ret r
+  case ιl => exact .ιl r
+  case ιr => exact .ιr r
+  case π1 => exact .π1 .prod r
+  case π2 => exact .π2 .prod r
+  case app ih =>
+    cases r with | β r₁ r₂ => exact .β (ih r₁) r₂
+  case letin ih =>
+    cases r with | ζ r₁ r₂ => exact .ζ (ih r₁) r₂
+  case fst ih =>
+    cases r with | π1 r₁ r₂ => exact .π1 (ih r₁) r₂
+  case snd ih =>
+    cases r with | π2 r₁ r₂ => exact .π2 (ih r₁) r₂
+
+theorem evalBigs {m n t} (r : m ⇒⋆ n) : n ⇓ t → m ⇓ t := by
+  induction r generalizing t <;> intro r
+  case refl => exact r
+  case trans r' _ ih => exact evalBig r' (ih r)
+
+theorem bigTerminal {t} (h : isTerminal t) : t ⇓ t := by
+  mutual_induction t generalizing h
+  all_goals simp at h
+  all_goals constructor
+
+theorem evalStep {m t} (h : isTerminal t) (r : m ⇒⋆ t) : ⟨m, []⟩ ⤳⋆ ⟨t, []⟩ :=
+  stepBig (evalBigs r (bigTerminal h))
